theories/typing/stype.v
@@ -14,15 +14,6 @@ Definition dual_action (a : action) : action :=
 Instance dual_action_involutive : Involutive (=) dual_action.
 Proof. by intros []. Qed.
 
-Class IsDualAction (a1 a2 : action) :=
-  is_dual_action : dual_action a1 = a2.
-Instance is_dual_action_default : IsDualAction a (dual_action a) | 100.
-Proof. done. Qed.
-Instance is_dual_action_Send : IsDualAction Send Receive.
-Proof. done. Qed.
-Instance is_dual_action_Receive : IsDualAction Receive Send.
-Proof. done. Qed.
-
 Inductive stype (V A : Type) :=
   | TEnd
   | TSR (a : action) (P : V → A) (st : V → stype V A).
@@ -53,7 +44,7 @@ Section stype_ofe.
        pointwise_relation V (≡) st1 st2 →
        TSR a P1 st1 ≡ TSR a P2 st2.
   Existing Instance stype_equiv.
-    
+
   Inductive stype_dist' (n : nat) : relation (stype V A) :=
     | TEnd_dist : stype_dist' n TEnd TEnd
     | TSR_dist a P1 P2 st1 st2 :
@@ -227,20 +218,29 @@ Proof.
   by intros ? A1 A2 B1 B2 n f g Hfg; apply stypeC_map_ne, cFunctor_contractive.
 Qed.
 
-Class IsDualStype {V} {A : ofeT} (st1 st2 : stype V A) :=
-  is_dual_stype : dual_stype st1 ≡ st2.
+Class IsDualAction (a1 a2 : action) :=
+  is_dual_action : dual_action a1 = a2.
+Instance is_dual_action_default : IsDualAction a (dual_action a) | 100.
+Proof. done. Qed.
+Instance is_dual_action_Send : IsDualAction Send Receive.
+Proof. done. Qed.
+Instance is_dual_action_Receive : IsDualAction Receive Send.
+Proof. done. Qed.
 
 Section DualStype.
-  Context `{PROP: bi} {V : Type}.
+  Context {V : Type} {A : ofeT}.
 
-  Global Instance is_dual_default (st : stype V PROP) :
+  Class IsDualStype (st1 st2 : stype V A) :=
+  is_dual_stype : dual_stype st1 ≡ st2.
+
+  Global Instance is_dual_default (st : stype V A) :
     IsDualStype st (dual_stype st) | 100.
   Proof. by rewrite /IsDualStype. Qed.
 
-  Global Instance is_dual_end : IsDualStype (TEnd : stype V PROP) TEnd.
+  Global Instance is_dual_end : IsDualStype (TEnd : stype V A) TEnd.
   Proof. constructor. Qed.
 
-  Global Instance is_dual_tsr a1 a2 P (st1 st2 : V → stype V PROP) :
+  Global Instance is_dual_tsr a1 a2 P (st1 st2 : V → stype V A) :
     IsDualAction a1 a2 →
     (∀ x, IsDualStype (st1 x) (st2 x)) →
     IsDualStype (TSR a1 P st1) (TSR a2 P st2).
@@ -248,15 +248,5 @@ Section DualStype.
     rewrite /IsDualAction /IsDualStype. intros <- Hst.
     by constructor=> x.
   Qed.
-  
-  Global Instance is_dual_send P (st1 st2 : V → stype V PROP) :
-    (∀ x, IsDualStype (st1 x) (st2 x)) →
-    IsDualStype (TSR Send P st1) (TSR Receive P st2).
-  Proof. intros H. by apply is_dual_tsr. Qed.
-  
-  Global Instance is_dual_receive P (st1 st2 : V → stype V PROP) :
-    (∀ x, IsDualStype (st1 x) (st2 x)) →
-    IsDualStype (TSR Receive P st1) (TSR Send P st2).
-  Proof. intros H. by apply is_dual_tsr. Qed.
 
 End DualStype.
