theories/examples/proofs_enc.v
@@ -10,24 +10,20 @@ Section ExampleProofsEnc.
   Context `{!heapG Σ} (N : namespace).
   Context `{!logrelG val Σ}.
 
-  Notation "⟦ c @ s : sτ ⟧{ γ }" := (interp_st N γ sτ c s)
-    (at level 10, s at next level, sτ at next level, γ at next level,
-     format "⟦  c  @  s  :  sτ  ⟧{ γ }").
-  
   Lemma seq_proof :
     {{{ True }}} seq_example {{{ v, RET v; ⌜v = #5⌝ }}}.
   Proof.
     iIntros (Φ H) "HΦ".
     rewrite /seq_example.
     wp_apply (new_chan_st_spec N
-             (TSend (λ v, ⌜v = 5⌝%I) (λ v, TEnd)))=> //.
+             (TSend (λ v, ⌜v = 5⌝%I) (λ v, TEnd)))=> //;
     iIntros (c γ) "[Hstl Hstr]"=> /=.
     wp_apply (send_st_spec N Z with "[$Hstl //]");
     iIntros "Hstl".
     wp_apply (recv_st_spec N Z with "[Hstr]"). iApply "Hstr".
     iIntros (v) "[Hstr HP]".
     iApply "HΦ".
-    iDestruct "HP" as %->.    
+    iDestruct "HP" as %->.
     eauto.
   Qed.
 
@@ -92,7 +88,7 @@ Section ExampleProofsEnc.
       (TSend (λ v, ∃ γ, ⟦ v @ Right :
         (TReceive
           (λ v, ⌜v = 5⌝)
-          (λ _, TEnd)) ⟧{γ})%I
+          (λ _, TEnd)) ⟧{N, γ})%I
       (λ v, TEnd)))=> //;
     iIntros (c γ) "[Hstl Hstr]"=> /=.
     wp_apply (wp_fork with "[Hstl]").
@@ -123,9 +119,9 @@ Section ExampleProofsEnc.
     wp_apply (new_chan_st_spec N
                (TSend (λ v, ⌜v = 5⌝%I) (λ v, TEnd)))=> //;
     iIntros (c γ) "[Hstl Hstr]"=> /=.
-    wp_apply (recv_st_spec _ with "Hstr");
+    wp_apply (recv_st_spec N Z with "Hstr");
     iIntros (v) "[Hstr HP]".
-    wp_apply (send_st_spec N with "[$Hstl //]");
+    wp_apply (send_st_spec N Z with "[$Hstl //]");
     iIntros "Hstl".
     iDestruct "HP" as %->.
     wp_pures.
@@ -161,10 +157,10 @@ Section ExampleProofsEnc.
     wp_apply (wp_fork with "[Hstr Hstr']").
     - iNext. wp_apply (recv_st_spec _ with "Hstr");
       iIntros (v) "[Hstr HP]".
-      wp_apply (send_st_spec _ with "[$Hstr' //]"). eauto.
-    - wp_apply (recv_st_spec _ with "[$Hstl' //]");
+      wp_apply (send_st_spec _ Z with "[$Hstr' //]"). eauto.
+    - wp_apply (recv_st_spec _ Z with "[$Hstl' //]");
       iIntros (v) "[Hstl' HP]".
-      wp_apply (send_st_spec _ with "[$Hstl //]");
+      wp_apply (send_st_spec _ Z with "[$Hstl //]");
       iIntros "Hstl".
       by iApply "HΦ".
   Qed.
